---
title: "STAT540-HW2-Problem1 & 2"
author: "Yunyi Lin/Pei Zeng"
date: "2/1/2018"
output: word_document
---

```{r setup, include=FALSE}
knitr::opts_chunk$set(echo = TRUE)
```
#Problem1
##a)  
$g(z) = \frac{1}{1+e^{-z}}$
Therefore,  
$\frac{\partial(g(z))}{\partial(z)} = \frac{0-(-e^{-z})}{(1+e^{-z})^2} = \frac{1}{1+e^{-z}}(\frac{1+e^{-z}-1}{1+e^{-z}}) = g(z)(1-g(z))$

##b)
$NLL(\theta) = -logP(D\mid\theta) = \sum_{i=1}^{n}[-y^{(i)}logh_{\theta}(x^{(i)})-(1-y^{(i)})log(1-h_{\theta}(x^{(i)}))]$  
$h_{\theta}(x^{(i)}) = g(\theta^Tx^{(i)}) = \frac{1}{1+e^{-\theta^Tx^{(i)}}}$  
Let $z = \theta^Tx^{(i)}$  
Then $\frac{\partial(NLL(\theta))}{\partial(\theta)} = \frac{\partial(NLL(\theta))}{\partial(z)}\frac{\partial(z)}{\partial(\theta)}$  
$\frac{\partial(z)}{\partial(\theta)} = \frac{\partial(\theta^Tx^{(i)})}{\partial(\theta)} = x^{(i)}$  
$\frac{\partial(NLL(\theta))}{\partial(z)} = \sum_{i=1}^{n}(-y^{(i)}\frac{(g(z)^{'})}{g(z)}-(1-y^{(i)})\frac{(1-g(z))^{'}}{1-g(z)}) = \sum_{i=1}^{n}(-y^{(i)}\frac{g(z)(1-g(z))}{g(z)}-(1-y^{(i)})\frac{g(z)(g(z)-1)}{(1-g(z))}) = \sum_{i=1}^{n}(-y^{(i)}+y^{(i)}g(z)-y^{(i)}g(z)+g(z)) = \sum_{i=1}^{n}(h_{\theta}(x^{(i)}-y^{(i)})$  
$\frac{\partial(NLL(\theta))}{\partial(\theta)} = \sum_{i=1}^{n}(h_{\theta}(x^{(i)}-y^{(i)})x^{(i)}$

##c)
$H = X^TSX$  
$S = diag(h_{\theta}(x^{(1)}(1-h_{\theta}(x^{(1)})),...,h_{\theta}(x^{(m)}(1-h_{\theta}(x^{(m)})))$  
$0<h_{\theta}(x^{(i)}(1-h_{\theta}(x^{(i)}))<1$  
$z^T_{1*d}H_{d*d}z_{d*1} = z^T_{1*d}(X^T_{d*m}S_{m*m}X_{m*d})z_{d*1} = (Xz)^TS(Xz) =$  
$(\sum_{j=1}^{n}x_j^{(1)}z_j)^2S_{11}+,...,+(\sum_{j=1}^{n}x_j^{(m)}z_j)^2S_{mm} = \sum_{i=1}^{n}S_{ii}(\sum_{j=1}^{n}x_j^{(i)}z_j)^2$
